Examples/Demo.lean
@@ -1,0 +1,87 @@
+import LeanBoogie.ITree
+import LeanBoogie.Util
+import LeanBoogie.Boogie
+
+#check 1
+open LeanBoogie
+
+-- # Coinduction, Interaction Trees
+
+inductive Delay' (A : Type) : Type
+| ret : A        -> Delay' A
+| tau : Delay' A -> Delay' A
+-- _Problem_: This is always finite
+-- def spin' : Delay' A := Delay'.tau spin' -- fails
+
+codata Delay A where
+| ret : A       -> Delay A
+| tau : Delay A -> Delay A
+
+def spin : Delay A := MvQPF.Cofix.corec (fun s => .tau s) 0 -- :)
+
+codata ITree_ E A where
+| ret : A          -> ITree_ E A
+| tau : ITree_ E A -> ITree_ E A
+| vis : E → (Int → ITree_ E A) → ITree_ E A
+--            ^^^ hard-coded answer type for now, due to limitation with QPFTypes
+
+/-- _Equivalence up to tau_. Notation: `~~` -/
+inductive Eutt_ : ITree E A → ITree E A → Prop
+| ret : Eutt_ (.ret r) (.ret r)
+| vis : (∀ a, Eutt (k₁ a) (k₂ a)) → Eutt_ (.vis e k₁) (.vis e k₂)
+| tau  : Eutt x y → Eutt_ (.tau x) (.tau y)
+| taul : Eutt x y → Eutt_ (.tau x) y
+| taur : Eutt x y → Eutt_ x (.tau y)
+
+/-
+  # ITrees form an (iterative) monad
+  These are our three central primitives
+-/
+def pure (a : A) : ITree E A                                                                        := ITree.ret a
+def bind (ta : ITree E A) (tb : A -> ITree E B) : ITree E B                                         := ITree.bind ta tb
+def iter (body : A -> ITree E (A ⊕ B)) (a₀ : A) : ITree E B                                         := sorry
+
+theorem iter_fp {f : A -> ITree E (A ⊕ B)} {a : A}
+  :  iter f a
+  = f a >>= (fun
+               | .inl a => iter f a -- continue
+               | .inr b => return b -- stop iterating
+             )
+  := ITree.trustITree "ITree paper page 9"
+
+/- # Memory
+
+  `ITree MemEv A`      ---(interp)--->      `S -> ITree Empty (A × S)`
+-/
+
+inductive MemEv /- Type -> -/ : Type where
+| read  : String        -> MemEv /- Int -/
+| write : String -> Int -> MemEv /- Unit -/
+
+def Mem.read  (v : String)             : ITree MemEv Int  := .vis (.read v)      (fun (ans : Int) => .ret ans)
+def Mem.write (v : String) (val : Int) : ITree MemEv Unit := .vis (.write v val) (fun (_unit : _) => .ret ())
+
+def BoogieState_ : Type := String -> Int
+-- def St_           (A : Type) : Type := BoogieState ->         (A × BoogieState)
+def Boogie_ (E : Type) (A : Type) : Type := BoogieState -> ITree E (A × BoogieState)
+
+def interp (tm : ITree MemEv A) : Boogie A := fun s₀ =>
+  ITree.corec (fun ⟨tm, s⟩ =>
+    match tm.dest with
+    | .ret a => .ret (a, s)
+    | .tau t => .tau (t, s)
+    | .vis (.read v) k => .tau ⟨k (s v), s⟩
+    | .vis (.write v val) k => .tau ⟨k (default), s.update v val⟩
+  ) (tm, s₀)
+
+theorem interp_pure : interp (ITree.pure x) = Boogie.pure x := sorry!
+--                                            ^^^^^^^^^^^ : `BoogieState -> ITree Empty (A × BoogieState)`
+--                            ^^^^^^^^^^^^ : `ITree MemEv A`
+
+theorem interp_bind {ta : ITree MemEv A} {tb : A -> ITree MemEv B}
+  : interp (ITree.bind ta tb)       =      Boogie.bind (interp ta) (fun a => interp (tb a))
+  := sorry!
+
+theorem interp_iter {body : A -> ITree MemEv (A ⊕ B)} {a₀ : A}
+  : interp (ITree.iter body a₀)    =       Boogie.iter (fun (a : A) => interp (body a)) a₀
+  := sorry!
