Examples/SimpleBlocky.lean
@@ -1,11 +1,11 @@
-import LeanBoogie.BoogieDsl
+import LeanBoogie.Dsl
 import LeanBoogie.ITree
-import LeanBoogie.Boog
+import LeanBoogie.Boogie
 import LeanBoogie.Mem
 import Auto
 import Aesop
 
-open Boogie ITree
+open LeanBoogie ITree
 
 set_option auto.smt true
 set_option trace.auto.smt.printCommands true
@@ -40,7 +40,7 @@ def p1 : ITree MemEv Unit := ITree.iter blocks 0
   | 2 => bb2
   | 3 => bb3
 
-procedure p2(x: int) {
+blocky_procedure p2(x: int) {
   var i: int;
   bb0:
     i := 0;
@@ -61,20 +61,20 @@ procedure p2(x: int) {
 -- For our boogie programs, `A` will usually be the label, and `B` will be `Unit`.
 theorem iter_fp {f : A -> ITree E (A ⊕ B)}
   : iter f a
-  ~~ f a >>= (match . with | .inl a => iter f a | .inr b => return b)
+  = f a >>= (match . with | .inl a => iter f a | .inr b => return b)
   := sorry
 
 -- set_option pp.notation false in
-example : EuttB (interp p1) (interp p2) := by
+example : interp p1 = interp p2 := by
   rw [p1]
 
   -- unroll once. bb0 always jumps to bb1 so this doesn't branch.
-  rw [iter_fp.eq];
+  rw [iter_fp];
   rw [p1.blocks, bb0];
   simp only [Fin.isValue, bind_assoc, pure_bind]
 
   -- unroll once again (bb1). This time we'll have to branch (see next comment)
-  rw [iter_fp.eq]; rw [p1.blocks, bb1];
+  rw [iter_fp]; rw [p1.blocks, bb1];
   simp only [Fin.isValue, ite_bind, bind_assoc, pure_bind]
   /- Now, we need to decide which block to jump to. In this case, we actually have enough information
     to know this, we know that `i < 3` in the following is true. But we need to interpret the memory
@@ -86,45 +86,46 @@ example : EuttB (interp p1) (interp p2) := by
     ```
     So let's push `interp` inwards, and decide which branch to take.
   -/
-  simp only [interp_bind.eq, interp_read.eq, interp_write.eq, interp_ite.eq] -- push `interp` inside
-  intro σ
-  simp only [Eutt.eq Boog.bind_push_state, Eutt.eq Boog.ite_push_state] -- push `σ` inside
-  simp only [Boog.read, Boog.write, BoogieState.update.eq_unfold] -- ! while this works, we should maybe try to avoid looking at the state `σ` ?
+  simp only [interp_bind, interp_read, interp_write, interp_ite] -- push `interp` inside
+  ext σ -- intro σ
+  dsimp [StateT.run]
+  simp only [Boogie.bind_push_state, Boogie.ite_push_state] -- push `σ` inside
+  simp only [Boogie.read, Boogie.write, BoogieState.update.eq_unfold] -- ! while this works, we should maybe try to avoid looking at the state `σ` ?
   simp
   -- Now our lhs is `interp (iter p1.blocks 2) σ'`, where we know that `σ' "i" = 0`. And we know that the next block is `bb2`.
 
   try
     -- Unroll twice (-> bb2, -> bb1)
-    rw [iter_fp.eq]; rw [p1.blocks, bb2]; simp only [Fin.isValue, ite_bind, bind_assoc, pure_bind]
-    rw [iter_fp.eq]; rw [p1.blocks, bb1]; simp only [Fin.isValue, ite_bind, bind_assoc, pure_bind]
+    rw [iter_fp]; rw [p1.blocks, bb2]; simp only [Fin.isValue, ite_bind, bind_assoc, pure_bind]
+    rw [iter_fp]; rw [p1.blocks, bb1]; simp only [Fin.isValue, ite_bind, bind_assoc, pure_bind]
     simp [Mem.update, bind_assoc]
-    simp only [interp_bind.eq, interp_read.eq, interp_write.eq, interp_ite.eq] -- push `interp` inside
-    simp only [Eutt.eq Boog.bind_push_state, Eutt.eq Boog.ite_push_state] -- push `σ` inside
-    simp [Boog.read, Boog.write, BoogieState.update.eq_unfold] -- "run" the straightline code -- ! while this works, we should maybe try to avoid looking at the state `σ` ?
+    simp only [interp_bind, interp_read, interp_write, interp_ite] -- push `interp` inside
+    simp only [Boogie.bind_push_state, Boogie.ite_push_state] -- push `σ` inside
+    simp [Boogie.read, Boogie.write, BoogieState.update.eq_unfold] -- "run" the straightline code -- ! while this works, we should maybe try to avoid looking at the state `σ` ?
 
   try
     -- Unroll twice (-> bb2, -> bb1)
-    rw [iter_fp.eq]; rw [p1.blocks, bb2]; simp only [Fin.isValue, ite_bind, bind_assoc, pure_bind]
-    rw [iter_fp.eq]; rw [p1.blocks, bb1]; simp only [Fin.isValue, ite_bind, bind_assoc, pure_bind]
+    rw [iter_fp]; rw [p1.blocks, bb2]; simp only [Fin.isValue, ite_bind, bind_assoc, pure_bind]
+    rw [iter_fp]; rw [p1.blocks, bb1]; simp only [Fin.isValue, ite_bind, bind_assoc, pure_bind]
     simp [Mem.update, bind_assoc]
-    simp only [interp_bind.eq, interp_read.eq, interp_write.eq, interp_ite.eq] -- push `interp` inside
-    simp only [Eutt.eq Boog.bind_push_state, Eutt.eq Boog.ite_push_state] -- push `σ` inside
-    simp [Boog.read, Boog.write, BoogieState.update.eq_unfold] -- "run" the straightline code -- ! while this works, we should maybe try to avoid looking at the state `σ` ?
+    simp only [interp_bind, interp_read, interp_write, interp_ite] -- push `interp` inside
+    simp only [Boogie.bind_push_state, Boogie.ite_push_state] -- push `σ` inside
+    simp [Boogie.read, Boogie.write, BoogieState.update.eq_unfold] -- "run" the straightline code -- ! while this works, we should maybe try to avoid looking at the state `σ` ?
 
   try
     -- Unroll twice (-> bb2, -> bb1)
-    rw [iter_fp.eq]; rw [p1.blocks, bb2]; simp only [Fin.isValue, ite_bind, bind_assoc, pure_bind]
-    rw [iter_fp.eq]; rw [p1.blocks, bb1]; simp only [Fin.isValue, ite_bind, bind_assoc, pure_bind]
+    rw [iter_fp]; rw [p1.blocks, bb2]; simp only [Fin.isValue, ite_bind, bind_assoc, pure_bind]
+    rw [iter_fp]; rw [p1.blocks, bb1]; simp only [Fin.isValue, ite_bind, bind_assoc, pure_bind]
     simp [Mem.update, bind_assoc]
-    simp only [interp_bind.eq, interp_read.eq, interp_write.eq, interp_ite.eq] -- push `interp` inside
-    simp only [Eutt.eq Boog.bind_push_state, Eutt.eq Boog.ite_push_state] -- push `σ` inside
-    simp [Boog.read, Boog.write, BoogieState.update.eq_unfold] -- "run" the straightline code -- ! while this works, we should maybe try to avoid looking at the state `σ` ?
+    simp only [interp_bind, interp_read, interp_write, interp_ite] -- push `interp` inside
+    simp only [Boogie.bind_push_state, Boogie.ite_push_state] -- push `σ` inside
+    simp [Boogie.read, Boogie.write, BoogieState.update.eq_unfold] -- "run" the straightline code -- ! while this works, we should maybe try to avoid looking at the state `σ` ?
 
   -- Unroll once (-> bb3, the final block)
-  rw [iter_fp.eq]; rw [p1.blocks, bb3]; simp only [Fin.isValue, ite_bind, bind_assoc, pure_bind]
-  simp only [interp_pure.eq, interp_bind.eq, interp_read.eq, interp_write.eq, interp_ite.eq] -- push `interp` inside
-  simp only [Boog.bind_push_state.eq, Boog.ite_push_state.eq] -- push `σ` inside
-  simp [Boog.read, Boog.write, BoogieState.update.eq_unfold] -- "run" the straightline code -- ! while this works, we should maybe try to avoid looking at the state `σ` ?
+  rw [iter_fp]; rw [p1.blocks, bb3]; simp only [Fin.isValue, ite_bind, bind_assoc, pure_bind]
+  simp only [interp_pure, interp_bind, interp_read, interp_write, interp_ite] -- push `interp` inside
+  simp only [Boogie.bind_push_state, Boogie.ite_push_state] -- push `σ` inside
+  simp [Boogie.read, Boogie.write, BoogieState.update.eq_unfold] -- "run" the straightline code -- ! while this works, we should maybe try to avoid looking at the state `σ` ?
   simp_all only [↓reduceIte]
 
   -- # Now, p2
@@ -132,9 +133,9 @@ example : EuttB (interp p1) (interp p2) := by
   simp [ITree.seq]
 
   -- unroll once
-  rw [iter_fp.eq]
+  rw [iter_fp]
   simp? [selectBlock]
-  rw [iter_fp.eq]
+  rw [iter_fp]
   simp? [selectBlock]
 
   sorry
