Examples/SimpleIterDijkstra.lean
@@ -1,0 +1,74 @@
+-- import LeanBoogie.BoogieDsl
+import LeanBoogie.ITree
+import LeanBoogie.ITree.ITree0W
+import LeanBoogie.Boogie
+import LeanBoogie.Woogie
+import LeanBoogie.Mem
+import Auto
+import Aesop
+
+open LeanBoogie
+open ITree
+
+set_option auto.smt true
+set_option trace.auto.smt.printCommands true
+set_option trace.auto.smt.result true
+set_option trace.auto.printLemmas true
+set_option auto.smt.trust true
+set_option auto.smt.solver.name "z3"
+set_option pp.fieldNotation.generalized false
+
+-- Very simple example which can be proven using unrolling or a congruence on the while loop
+
+def p1 : ITree MemEv Unit := do
+  Mem.write "i" 0
+  while_ (return (<- Mem.read "i") < 1) do
+    Mem.update "i" (. + 1)
+    Mem.update "x" (. + 2)
+  Mem.write "i" 0 -- need to set `i` to 0 afterwards, otherwise the programs compute the same `x` but not `i`.
+
+def p2 : ITree MemEv Unit := do
+  Mem.write "i" 0
+  while_ (return (<- Mem.read "i") < 2) do
+    Mem.update "x" (. + 1)
+    Mem.update "i" (. + 1)
+  Mem.write "i" 0
+
+theorem StateT.bind_push_state [Monad M] [LawfulMonad M] {a : StateT S M A} {b : A -> StateT S M B} : (a >>= b) σ = (a σ >>= fun res => b res.fst res.snd) := rfl
+theorem Woogie.bind_push_state {a : Woogie A} {b : A -> Woogie B} : (a >>= b) σ = (a σ >>= fun res => b res.fst res.snd) := rfl
+theorem Woogie.ite_push_state [Decidable c] {t e : Woogie A} : (if c then t else e) σ = (if c then t σ else e σ) := by aesop
+theorem ITree0W.bind_push_fst {wa : ITree0W A} {wb : A -> ITree0W B}
+  : (wa >>= wb).fst
+  = (fun post => wa.fst (fun ta => (∃ a, Converges a ta ∧ (wb a).fst post) ∨ Diverges ta))
+  := rfl
+
+
+set_option maxHeartbeats 10000000
+set_option pp.fieldNotation false in
+example : θ (interp p1) <= θ (interp p2) := by
+  rw [p1, p2]
+  conv => lhs; rw [while_unroll1, while_unroll1, ]; simp
+  conv => rhs; rw [while_unroll1, while_unroll1, while_unroll1]; simp
+  simp [interp_bind, interp_write, interp_ite, interp_pure,
+    Mem.update, interp_write, interp_read, ITree.skip]
+
+  simp [θ_bind, Woogie.θ_read, Woogie.θ_write, Woogie.θ_ite] at * -- thread theta through
+
+  intro s post hp
+  simp [Woogie.bind_push_state, Woogie.ite_push_state] at *
+
+  dsimp [Pure.pure, Bind.bind] at *
+  unfold ITree0W.bind at *
+  simp
+  -- ∃ a, Converges a ta ∧ ...
+  -- ! assuming converges tw >>= ...
+  unfold Woogie.write at *
+  unfold Woogie.read at *
+  unfold BoogieState.update at *
+  simp at *
+
+  simp [Converges.eq_unfold, Diverges.eq_unfold] at *
+  sorry
+  done
+
+#check 1
